Language.v
@@ -16,10 +16,13 @@ Inductive bexp : Type :=
 
 Inductive com : Type :=
   | CSkip : com
-  | CSeq : com -> com -> com.
+  | CSeq : com -> com -> com
+  | CAss : string -> aexp -> com. 
 
 Bind Scope com_scope with com.
 Notation "'SKIP'" :=
      CSkip : com_scope.
 Notation "c1 ;; c2" :=
     (CSeq c1 c2) (at level 80, right associativity) : com_scope.
+Notation "x '::=' a" :=
+    (CAss x a) (at level 60) : com_scope.
