practice.v
@@ -30,32 +30,44 @@ Lemma abstract_aexp_mult_sound : forall ast st e1 e2,
 Proof. intros. simpl. apply gamma_distr_mult; assumption.
 Qed.
 
-Theorem abstract_aexp_eval_sound : forall ast st e,
-  (forall x, gamma (ast x) (st x)) ->
+Lemma abstract_aexp_var_sound : forall ast st x,
+  gamma (ast x) (st x) -> 
+  gamma (abstract_eval_aexp ast (AVar x)) (eval_aexp st (AVar x)).
+Proof. intros. simpl. assumption. Qed.
+
+Theorem abstract_aexp_eval_sound : forall ast x st e,
+  gamma (ast x) (st x) ->
   (gamma (abstract_eval_aexp ast e)) (eval_aexp st e).
 Proof.
   induction e; intros.
-  - (* ANum *)
-    simpl. apply gamma_extract_n_n.
-  - (* AVar *)
-    simpl. apply H.
-  - (* APlus *)
-    apply abstract_aexp_plus_sound; auto.
-  - (* AMult *)
-    apply abstract_aexp_mult_sound; auto.
+  - (* ANum *) simpl. apply gamma_extract_n_n.
+  - (* AVar *) apply abstract_aexp_var_sound. admit.
+
+  - (* APlus *) apply abstract_aexp_plus_sound; auto.
+  - (* AMult *) apply abstract_aexp_mult_sound; auto.
+Admitted.
+
+Lemma abstract_ceval_ass_sound : forall ast x st a,
+  gamma (ast x) (st x) ->
+  gamma (ceval_abstract ast (x ::= a) x) (ceval st (x ::= a) x).
+Proof.
+  intros. simpl. unfold t_update.  rewrite <- beq_string_refl.
+  apply abstract_aexp_eval_sound with (x:=x). assumption.
 Qed.
 
 Lemma abstract_ceval_seq_sound : forall ast c1 c2 x st,
   gamma ((ceval_abstract ast c1) x) ((ceval st c1) x) ->
   gamma (ceval_abstract ast (c1;; c2) x) (ceval st (c1;; c2) x).
 Proof.
-   intros. generalize dependent c1. induction c2; intros.
-   - auto.
-   - replace (ceval_abstract ast (c1;; c2_1;; c2_2))
-     with (ceval_abstract ast ((c1;; c2_1);; c2_2)).
-     apply IHc2_2. apply IHc2_1. assumption.
-     reflexivity.
-Qed.
+  intros. generalize dependent c1. induction c2; intros.
+  - (* CSkip *) simpl. apply H.
+  - (* CSeq  *) replace (ceval_abstract ast (c1;; c2_1;; c2_2)) with
+    (ceval_abstract ast ((c1;; c2_1);;c2_2)); try reflexivity. 
+    replace (ceval st (c1;; c2_1 ;; c2_2)) with
+      (ceval st ((c1 ;; c2_1) ;; c2_2)); try reflexivity.
+      apply IHc2_2.  apply IHc2_1. apply H.
+  - (* CAss *) simpl. admit.
+Admitted.
 
 Theorem abstract_ceval_sound : forall ast st c x,
   (forall x, gamma (ast x) (st x)) ->
@@ -66,7 +78,8 @@ Proof.
     intros. simpl. apply H.
   - (* CSeq *)
     apply abstract_ceval_seq_sound. assumption.
-Qed.
+  - admit.
+Admitted.
     
 
 
